Add initial model functions

CPL_Utils.thy
@@ -2,6 +2,14 @@ theory "CPL_Utils"
   imports Main "CPL_Instance"
 begin
 
+(* ================= Extra Utility Functions ================= *)
+
+fun setToList :: "'a set \<Rightarrow> 'a list" where
+"setToList S = (SOME l. set l = S)" (*Ref: https://stackoverflow.com/a/28636535*)
+
+lemma set_set_to_list : "finite S \<Longrightarrow> set (setToList S) = S"
+  by (metis (mono_tags, lifting) finite_list setToList.simps someI_ex)
+
 (* ================= Proof System Utility Functions ================= *)
 
 (* Note: |` is called restrict_map operator. m |` A = (\<lambda>x. if x \<in> A then m x else None) *)
@@ -23,6 +31,9 @@ fun allMaps :: "nat \<Rightarrow> Variable set \<Rightarrow> 'a set \<Rightarrow
 fun buildValuation :: "Variable list \<Rightarrow> 'a list \<Rightarrow> 'a Valuation"  where
 "buildValuation [] [] = Map.empty " |
 "buildValuation variables values = Map.empty (variables [\<mapsto>] values)"
+
+fun HOmap :: "'a Valuation \<Rightarrow> Variable list \<Rightarrow> 'a list" where
+"HOmap f var_list = [the (f v). v \<leftarrow> var_list, (f v) \<noteq> None, (v \<in> (dom f))]"
 
 fun isParent :: "'a Judgement \<Rightarrow> 'a Judgement \<Rightarrow> Formula \<Rightarrow> bool" where
 "isParent \<J>\<^sub>1 \<J>\<^sub>2 \<phi> = (
@@ -51,6 +62,10 @@ fun isParent :: "'a Judgement \<Rightarrow> 'a Judgement \<Rightarrow> Formula \
     )
   )
 )"
+
+fun existSq :: "Variable list \<Rightarrow> Formula \<Rightarrow> Formula" where
+"existSq [] \<phi> = \<phi>" |
+"existSq (v#vs) \<phi> = (Exists v (existSq vs \<phi>))"
 
 (* ======================== Tests ======================== *)
 
